@prefix : <https://gis.lu.se/ont/context#> .
@prefix owl: <http://www.w3.org/2002/07/owl#> .
@prefix rdf: <http://www.w3.org/1999/02/22-rdf-syntax-ns#> .
@prefix xml: <http://www.w3.org/XML/1998/namespace> .
@prefix xsd: <http://www.w3.org/2001/XMLSchema#> .
@prefix rdfs: <http://www.w3.org/2000/01/rdf-schema#> .
@base <https://gis.lu.se/ont/context> .

<https://gis.lu.se/ont/context> rdf:type owl:Ontology ;
                                 rdfs:label "Visualisation context vocabulary"@en ;
                                 rdfs:comment """This file is created by:
Weiming Huang
GIS Centre
Lund University
weiming.huang@nateko.lu.se"""@en .

#################################################################
#    Object Properties
#################################################################

###  https://gis.lu.se/ont/context#hasVisualisationPhenomenon
:hasVisualisationPhenomenon rdf:type owl:ObjectProperty ;
                            rdfs:domain :VisualisationContext .


#################################################################
#    Data properties
#################################################################

###  https://gis.lu.se/ont/context#hasVisualisationScale
:hasVisualisationScale rdf:type owl:DatatypeProperty ;
                       rdfs:domain :VisualisationContext ;
                       rdfs:range xsd:decimal ;
                       rdfs:comment "For associating a visualisation scale value, which should be a denominator of the scale value."@en .


#################################################################
#    Classes
#################################################################

###  https://gis.lu.se/ont/context#VisualisationContext
:VisualisationContext rdf:type owl:Class ;
                      rdfs:comment "Represents the visualisation context transferred from the visualisation clients, two types of information are modelled in this vocabulary, i.e. visualisation scale and phenomenon."@en .


###  Generated by the OWL API (version 4.2.8.20170104-2310) https://github.com/owlcs/owlapi
